Updating swap

MirrorCharge!/src/MirrorCharge/Java/TestPullConjunct.v
@@ -10,6 +10,7 @@ Require Import MirrorCharge.RTac.PullConjunct.
 
 Require Import MirrorCharge.ModularFunc.BaseFunc.
 Require Import MirrorCharge.ModularFunc.ILogicFunc.
+Require Import MirrorCharge.ModularFunc.BILogicFunc.
 Require Import MirrorCharge.ModularFunc.EmbedFunc.
 
 Require Import MirrorCore.Lambda.ExprCore.
@@ -23,11 +24,25 @@ Print rtac.
 
 Set Printing Width 140.
 
+Fixpoint seq_pc n : expr typ func :=
+  match n with
+    | 0 => mkAnd tyProp (mkTrue tyProp) (mkFalse tyProp)
+    | S n => mkAnd tyProp (seq_pc n) (seq_pc n)
+  end.
+
 Definition goal1 : expr typ func := mkEntails tyProp 
 	(mkAnd tyProp (mkTrue tyProp) (mkFalse tyProp)) (mkTrue tyProp).
 
 Definition goal2 : expr typ func := mkEntails tyProp 
 	(mkAnd tyProp (mkAnd tyProp (mkTrue tyProp) (mkFalse tyProp)) (mkAnd tyProp (mkAnd tyProp (mkFalse tyProp) (mkTrue tyProp)) (mkFalse tyProp))) (mkTrue tyProp).
 
+
+
 Eval vm_compute in PCT nil nil 0 0 CTop (@ctx_empty typ (expr typ func) subst SU CTop) goal1.
 Eval vm_compute in PCT nil nil 0 0 CTop (ctx_empty (expr := expr typ func) (subst := subst)) goal2.
+Example test : exists x, PCT nil nil 0 0 CTop (ctx_empty (expr := expr typ func) (subst := subst)) 
+	(mkEntails tyProp (mkAnd tyProp (seq_pc 1) (mkEmp tyProp)) (mkTrue tyProp)) = x.
+Proof.
+  simpl.
+  unfold pull_conjunct. simpl.
+  unfold sr_combine, il_respects, setoid_rewrite; simpl.
